reduce instr set, and proved more stuff

memory.v
@@ -7,26 +7,23 @@ Require Import Coq.Program.Equality.
 (** Memory model  *)
 Definition LocalMemory : Set := LocalVariable ⇀ RuntimeValue.
 
-Inductive local_mem_contains_r : LocalMemory → Resource → Set :=
-  | local_mem_contains_r_c : ∀ {L : LocalMemory} {x : LocalVariable } {r1 r2 : Resource},
-    maps_to L x r1 →
-    resource_contains_r r1 r2 →
-    local_mem_contains_r L r2
-.
-
 Inductive local_mem_contains_t : LocalMemory → Tag → Set :=
-  | local_mem_contains_tc : ∀ (L : LocalMemory) (x : LocalVariable) (r : Resource),
-    maps_to L x r → ∀ t,
+  | local_mem_contains_tc : ∀ {L : LocalMemory} {x : LocalVariable} {r : Resource},
+    maps_to L x r → ∀ {t},
     resource_contains_t r t →
     local_mem_contains_t L t
 .
 
-Lemma local_mem_contains_tc_inj : ∀ L x r t H p1 p2, local_mem_contains_tc L x r t H p1 = local_mem_contains_tc L x r t H p2 → p1 = p2.
-Proof.
-  intros.
-  dependent destruction H0.
-  reflexivity.
-Qed.
+Definition local_mem_remove (L : LocalMemory) x := remove L x.
+
+Definition GlobalMemory : Set := GlobalResourceID ⇀ Resource.
+
+Inductive global_mem_contains_t : GlobalMemory → Tag → Set :=
+  | global_mem_contains_rt : ∀ {G : GlobalMemory} {x : GlobalResourceID} {r},
+    maps_to G x r → ∀ {t},
+    resource_contains_t r t →
+    global_mem_contains_t G t
+.
 
 Module StructSig.
 Record StructSig := {
@@ -36,54 +33,100 @@ Record StructSig := {
 End StructSig.
 Import StructSig(StructSig).
 
-Record Module : Set := {
+Record ModuleDefinition : Set := {
   struct_decls : StructName ⇀ StructSig;
 }.
 
-Record Account : Set := {
-  resources : StructName ⇀ Resource;
-  modules : ModuleName ⇀ Module
-}.
-
-Definition GlobalMemory : Set := AccountAddress ⇀ Account.
-
-Inductive global_mem_contains_r : GlobalMemory → Resource → Set :=
-  | global_mem_contains_r_c : ∀ {G : GlobalMemory} {x : GlobalResourceID} {a} {r1 r2 : Resource},
-    maps_to G x.(mod_id).(account_addr) a →
-    maps_to a.(resources) x.(name) r1 →
-    resource_contains_r r1 r2 →
-    global_mem_contains_r G r2
-.
-
-Inductive global_mem_contains_t : GlobalMemory → Tag → Set :=
-  | global_mem_contains_rt : ∀ {G : GlobalMemory} {x : GlobalResourceID} {a} {r} {t},
-    maps_to G x.(mod_id).(account_addr) a →
-    maps_to a.(resources) x.(name) r →
-    resource_contains_t r t →
-    global_mem_contains_t G t
-.
+Definition ModuleDefinitions := (AccountAddress * ModuleName) ⇀ ModuleDefinition.
 
 Record Memory := {
   local: LocalMemory;
   global: GlobalMemory;
 }.
 
-Inductive mem_contains_r : Memory → Resource → Set :=
-  | local_mem_cr : ∀ {L} {G} {r}, local_mem_contains_r L r → mem_contains_r {|
-    local := L; global := G;
-  |} r
-  | global_mem_cr : ∀ {L} {G} {r}, global_mem_contains_r G r → mem_contains_r {|
-    local := L; global := G;
-  |} r
-.
-
 Inductive mem_contains_t : Memory → Tag → Set :=
-  | local_mem_ct : ∀ m t, local_mem_contains_t m.(local) t → mem_contains_t m t
-  | global_mem_ct : ∀ m t, global_mem_contains_t m.(global) t → mem_contains_t m t
+  | local_mem_ct : ∀ {m} {t}, local_mem_contains_t m.(local) t → mem_contains_t m t
+  | global_mem_ct : ∀ {m} {t}, global_mem_contains_t m.(global) t → mem_contains_t m t
 .
 
 Definition mem_remove (M : Memory) (x : LocalVariable) : Memory.
-Admitted.
+Proof.
+  destruct M as [local global].
+  constructor.
+  + refine (remove local x).
+  + refine global.
+Defined.
+
+Definition maps_var_to (M : Memory) x v : Set := maps_to M.(local) x v.
+
+Lemma remove_p1 : ∀ {Y : Set} (M : LocalVariable ⇀ Y) x v, notT (maps_to (remove M x) x v).
+Proof.
+  intros Y M x v Hc.
+  unfold remove in Hc.
+  unfold maps_to in Hc.
+  simpl in Hc.
+  destruct (var_dec_eq x x).
+  + inversion Hc.
+  + apply n. reflexivity.
+Qed.
+
+Lemma mem_remove_p1 : ∀ M x v, notT (maps_var_to (mem_remove M x) x v).
+Proof.
+  intros M x v Hc.
+  destruct M as [local global].
+  inversion Hc.
+  unfold remove in H0.
+  simpl in H0.
+  destruct (var_dec_eq x x).
+  + inversion H0.
+  + apply n. reflexivity.
+Qed.
+
+Lemma remove_p2 : ∀ {Y : Set} (M : LocalVariable ⇀ Y) x y v, ¬ x = y →  (maps_to (remove M x) y v) = (maps_to M y v).
+Proof.
+  intros Y M x y v H.
+  unfold remove.
+  unfold maps_to.
+  destruct (eq_dec y x); auto.
+  rewrite e in H.
+  contradiction.
+Qed.
+
+Lemma mem_remove_p2 : ∀ M x y v, ¬ x = y →  (maps_var_to (mem_remove M x) y v) = (maps_var_to M y v).
+Proof.
+  intros M x y v H.
+  destruct M as [local global].
+  unfold mem_remove.
+  unfold maps_var_to.
+  simpl.
+  unfold maps_to.
+  unfold remove.
+  destruct (eq_dec y x); auto.
+  rewrite e in H.
+  contradiction.
+Qed.
+
+Lemma remove_p3 : ∀ {Y : Set}  (M : LocalVariable ⇀ Y) x y v, (maps_to (remove M x) y v) → maps_to M y v.
+Proof.
+  intros Y M x y v H.
+  erewrite <- remove_p2.
+  + exact H.
+  + intro Hc.
+    rewrite Hc in H.
+    eapply remove_p1.
+    exact H.
+Qed.
+
+Lemma mem_remove_p3 : ∀ M x y v, (maps_var_to (mem_remove M x) y v) → maps_var_to M y v.
+Proof.
+  intros M x y v H.
+  erewrite <- mem_remove_p2.
+  + exact H.
+  + intro Hc.
+    rewrite Hc in H.
+    eapply mem_remove_p1.
+    exact H.
+Qed.
 
 Definition mem_update_local (M : Memory) (x : LocalVariable) (v : RuntimeValue) : Memory.
 Admitted.
@@ -105,32 +148,16 @@ Lemma mem_update_local_u2 {M} {x} {u : UnrestrictedValue} :
 ∀ t, local_mem_contains_t (mem_update_local M x u).(local) t → local_mem_contains_t M.(local) t.
 Admitted.
 
-Definition mem_update_ref (M : Memory) (r : Reference) (v : RuntimeValue) : Memory.
-Admitted.
+Inductive maps_struct_kind : ModuleDefinitions → StructType → Kind → Prop :=.
 
-Definition maps_var_to (M : Memory) x v : Set := maps_to M.(local) x v.
-
-Inductive maps_ref_to : Memory → Reference → RuntimeValue → Prop :=.
-
-Inductive maps_struct_kind : Memory → StructType → Kind → Prop :=.
-
-Inductive maps_struct_arity : Memory → StructType → nat → Prop :=.
+Inductive maps_struct_arity : ModuleDefinitions → StructType → nat → Prop :=.
 
 Definition LocalStack : Set := list RuntimeValue.
-
-Inductive lstack_contains_r : LocalStack → Resource → Set :=
-  | lstack_car : ∀ (r1 r2 : Resource) S,
-    resource_contains_r r1 r2 →
-    lstack_contains_r (val r1 :: S) r2
-  | lstack_cdr : ∀ v r S,
-    lstack_contains_r S r →
-    lstack_contains_r (v :: S) r
-.
 
 Inductive lstack_contains_t : LocalStack → Tag → Set :=
   | lstackt_car : ∀ S r t,
     resource_contains_t r t →
-    lstack_contains_t (val r :: S) t
+    lstack_contains_t (resourceValue r :: S) t
   | lstackt_cdr : ∀ S t,
     lstack_contains_t S t →
     ∀ v, lstack_contains_t (v :: S) t
