value.v
@@ -51,14 +51,6 @@ Coercion unsignedInt64Value : UnsignedInt64 >-> PrimitiveValue.
 Coercion accountAddressValue : AccountAddress >-> PrimitiveValue.
 Coercion bytesValue : Bytes >-> PrimitiveValue.
 
-Inductive resource_contains_r : Resource → Resource → Set :=
-  | rc_id : ∀ {r}, resource_contains_r r r
-  | rc_field : ∀ {t} {τ} {field_vals : list Value} {r1 r2 : Resource},
-    list_contains field_vals r1 →
-    resource_contains_r r1 r2 →
-    resource_contains_r (resource t τ field_vals) r2
-.
-
 Inductive resource_contains_t : Resource → Tag → Set :=
   | rct_root : ∀ {r}, resource_contains_t r (tag_of r)
   | rct_field : ∀ {t1 t2} {τ} {field_vals : list Value} {r : Resource},
@@ -67,68 +59,4 @@ Inductive resource_contains_t : Resource → Tag → Set :=
     resource_contains_t (resource t1 τ field_vals) t2
 .
 
-(** References  *)
-Inductive Qualifier : Set :=
-  | mut : Qualifier
-  | immut : Qualifier.
-
-Inductive Root : Set :=
-  | local_root : LocalVariable -> Root
-  | global_root : GlobalResourceID -> Root.
-
-Coercion local_root : LocalVariable >-> Root.
-Coercion global_root : GlobalResourceID >-> Root.
-
-Definition Path := list FieldName.
-
-Parameter read_val : Value → Path → Value → Prop.
-
-Axiom read_unrestricted : ∀ (u : UnrestrictedValue) (p : Path) (v : Value),
-  read_val u p v →
-  ∃ (u' : UnrestrictedValue), v = u'.
-
-Axiom read_resource : ∀ (s : Value) (p : Path) (a : Resource),
-read_val s p a →
-∃ (b : Resource), s = b.
-
-Record Reference : Set := {
-  root : Root;
-  access_path : Path;
-  mutability : Qualifier;
-}.
-
-Inductive is_mut : Reference → Prop :=
-  | is_mut_ref : ∀ (r : Root) (p : Path), is_mut {|
-    root := r; access_path := p; mutability := mut;
-  |}.
-
-Inductive is_immut : Reference → Prop :=
-  | is_immut_ref : ∀ (r : Root) (p : Path), is_immut {|
-  root := r; access_path := p; mutability := immut;
-  |}.
-
-Definition extend_ref (r : Reference) (e : FieldName) : Reference :=
-  match r with
-  | {| root := root ; access_path := access_path; mutability := mutability |} => {|
-    root := root;
-    access_path := access_path ++ [ e ];
-    mutability := mutability;
-  |}
-  end.
-
-Definition freeze_ref (r : Reference) : Reference :=
-  match r with
-  | {| root := root; access_path := access_path; mutability := _ |} => {|
-      root := root;
-      access_path := access_path;
-      mutability := immut;
-  |}
-  end.
-
-Inductive RuntimeValue : Set :=
-  | val : Value → RuntimeValue
-  | ref_val : Reference → RuntimeValue.
-
-Coercion val : Value >-> RuntimeValue.
-Coercion ref_val : Reference >-> RuntimeValue.
-Coercion foo (v : UnrestrictedValue) := val (unrestrictiveValue v).
+Definition RuntimeValue := Value.
